Compatibility fixes, backtrack on definitions of reflexive, symmetric... classes for now, merging Relations with RelationClasses requires some non-trivial changes on implicits but also some definitions are different (e.g. antisymmetric in Classes is defined w.r.t an equivalence relation and not eq). Move back to Reflexive and so on. reflexivity-like tactics fail in the same way as before if Setoid was not imported. There is now a scope for morphism signatures, hence "==>", "++>" and "-->" can be given different interpretations.
git-svn-id: svn+ssh://scm.gforge.inria.fr/svn/coq/trunk@10708 85f007b7-540e-0410-9357-904b9bb8a0f7

theories/Classes/RelationClasses.v
@@ -50,74 +50,74 @@ Proof. reflexivity. Qed.
 
 (** We rebind relations in separate classes to be able to overload each proof. *)
 
-Class reflexive A (R : relation A) :=
+Class Reflexive A (R : relation A) :=
   reflexivity : forall x, R x x.
 
-Class irreflexive A (R : relation A) := 
+Class Irreflexive A (R : relation A) := 
   irreflexivity : forall x, R x x -> False.
 
-Class symmetric A (R : relation A) := 
+Class Symmetric A (R : relation A) := 
   symmetry : forall x y, R x y -> R y x.
 
-Class asymmetric A (R : relation A) := 
+Class Asymmetric A (R : relation A) := 
   asymmetry : forall x y, R x y -> R y x -> False.
 
-Class transitive A (R : relation A) := 
+Class Transitive A (R : relation A) := 
   transitivity : forall x y z, R x y -> R y z -> R x z.
 
-Implicit Arguments reflexive [A].
-Implicit Arguments irreflexive [A].
-Implicit Arguments symmetric [A].
-Implicit Arguments asymmetric [A].
-Implicit Arguments transitive [A].
+Implicit Arguments Reflexive [A].
+Implicit Arguments Irreflexive [A].
+Implicit Arguments Symmetric [A].
+Implicit Arguments Asymmetric [A].
+Implicit Arguments Transitive [A].
 
 Hint Resolve @irreflexivity : ord.
 
 (** We can already dualize all these properties. *)
 
-Program Instance [ ! reflexive A R ] => flip_reflexive : reflexive (flip R) :=
+Program Instance [ ! Reflexive A R ] => flip_Reflexive : Reflexive (flip R) :=
   reflexivity := reflexivity (R:=R).
 
-Program Instance [ ! irreflexive A R ] => flip_irreflexive : irreflexive (flip R) :=
+Program Instance [ ! Irreflexive A R ] => flip_Irreflexive : Irreflexive (flip R) :=
   irreflexivity := irreflexivity (R:=R).
 
-Program Instance [ ! symmetric A R ] => flip_symmetric : symmetric (flip R).
+Program Instance [ ! Symmetric A R ] => flip_Symmetric : Symmetric (flip R).
 
-  Solve Obligations using unfold flip ; program_simpl ; clapply symmetric.
+  Solve Obligations using unfold flip ; program_simpl ; clapply Symmetric.
 
-Program Instance [ ! asymmetric A R ] => flip_asymmetric : asymmetric (flip R).
+Program Instance [ ! Asymmetric A R ] => flip_Asymmetric : Asymmetric (flip R).
   
   Solve Obligations using program_simpl ; unfold flip in * ; intros ; clapply asymmetry.
 
-Program Instance [ ! transitive A R ] => flip_transitive : transitive (flip R).
+Program Instance [ ! Transitive A R ] => flip_Transitive : Transitive (flip R).
 
   Solve Obligations using unfold flip ; program_simpl ; clapply transitivity.
 
 (** Have to do it again for Prop. *)
 
-Program Instance [ ! reflexive A (R : relation A) ] => inverse_reflexive : reflexive (inverse R) :=
+Program Instance [ ! Reflexive A (R : relation A) ] => inverse_Reflexive : Reflexive (inverse R) :=
   reflexivity := reflexivity (R:=R).
 
-Program Instance [ ! irreflexive A (R : relation A) ] => inverse_irreflexive : irreflexive (inverse R) :=
+Program Instance [ ! Irreflexive A (R : relation A) ] => inverse_Irreflexive : Irreflexive (inverse R) :=
   irreflexivity := irreflexivity (R:=R).
 
-Program Instance [ ! symmetric A (R : relation A) ] => inverse_symmetric : symmetric (inverse R).
+Program Instance [ ! Symmetric A (R : relation A) ] => inverse_Symmetric : Symmetric (inverse R).
 
-  Solve Obligations using unfold inverse, flip ; program_simpl ; clapply symmetric.
+  Solve Obligations using unfold inverse, flip ; program_simpl ; clapply Symmetric.
 
-Program Instance [ ! asymmetric A (R : relation A) ] => inverse_asymmetric : asymmetric (inverse R).
+Program Instance [ ! Asymmetric A (R : relation A) ] => inverse_Asymmetric : Asymmetric (inverse R).
   
   Solve Obligations using program_simpl ; unfold inverse, flip in * ; intros ; clapply asymmetry.
 
-Program Instance [ ! transitive A (R : relation A) ] => inverse_transitive : transitive (inverse R).
+Program Instance [ ! Transitive A (R : relation A) ] => inverse_Transitive : Transitive (inverse R).
 
   Solve Obligations using unfold inverse, flip ; program_simpl ; clapply transitivity.
 
-Program Instance [ ! reflexive A (R : relation A) ] => 
-  reflexive_complement_irreflexive : irreflexive (complement R).
+Program Instance [ ! Reflexive A (R : relation A) ] => 
+  Reflexive_complement_Irreflexive : Irreflexive (complement R).
 
-Program Instance [ ! irreflexive A (R : relation A) ] => 
-  irreflexive_complement_reflexive : reflexive (complement R).
+Program Instance [ ! Irreflexive A (R : relation A) ] => 
+  Irreflexive_complement_Reflexive : Reflexive (complement R).
 
   Next Obligation. 
   Proof. 
@@ -125,7 +125,7 @@ Program Instance [ ! irreflexive A (R : relation A) ] =>
     apply (irreflexivity H).
   Qed.
 
-Program Instance [ ! symmetric A (R : relation A) ] => complement_symmetric : symmetric (complement R).
+Program Instance [ ! Symmetric A (R : relation A) ] => complement_Symmetric : Symmetric (complement R).
 
   Next Obligation.
   Proof.
@@ -155,34 +155,34 @@ Ltac obligations_tactic ::= simpl_relation.
 
 (** Logical implication. *)
 
-Program Instance impl_refl : reflexive impl.
-Program Instance impl_trans : transitive impl.
+Program Instance impl_refl : Reflexive impl.
+Program Instance impl_trans : Transitive impl.
 
 (** Logical equivalence. *)
 
-Program Instance iff_refl : reflexive iff.
-Program Instance iff_sym : symmetric iff.
-Program Instance iff_trans : transitive iff.
+Program Instance iff_refl : Reflexive iff.
+Program Instance iff_sym : Symmetric iff.
+Program Instance iff_trans : Transitive iff.
 
 (** Leibniz equality. *)
 
-Program Instance eq_refl : reflexive (@eq A).
-Program Instance eq_sym : symmetric (@eq A).
-Program Instance eq_trans : transitive (@eq A).
+Program Instance eq_refl : Reflexive (@eq A).
+Program Instance eq_sym : Symmetric (@eq A).
+Program Instance eq_trans : Transitive (@eq A).
 
 (** Various combinations of reflexivity, symmetry and transitivity. *)
 
-(** A [PreOrder] is both reflexive and transitive. *)
+(** A [PreOrder] is both Reflexive and Transitive. *)
 
 Class PreOrder A (R : relation A) :=
-  preorder_refl :> reflexive R ;
-  preorder_trans :> transitive R.
+  preorder_refl :> Reflexive R ;
+  preorder_trans :> Transitive R.
 
-(** A partial equivalence relation is symmetric and transitive. *)
+(** A partial equivalence relation is Symmetric and Transitive. *)
 
 Class PER (carrier : Type) (pequiv : relation carrier) :=
-  per_sym :> symmetric pequiv ;
-  per_trans :> transitive pequiv.
+  per_sym :> Symmetric pequiv ;
+  per_trans :> Transitive pequiv.
 
 (** We can build a PER on the Coq function space if we have PERs on the domain and
    codomain. *)
@@ -201,20 +201,20 @@ Program Instance [ PER A (R : relation A), PER B (R' : relation B) ] =>
 (** The [Equivalence] typeclass. *)
 
 Class Equivalence (carrier : Type) (equiv : relation carrier) :=
-  equiv_refl :> reflexive equiv ;
-  equiv_sym :> symmetric equiv ;
-  equiv_trans :> transitive equiv.
+  equiv_refl :> Reflexive equiv ;
+  equiv_sym :> Symmetric equiv ;
+  equiv_trans :> Transitive equiv.
 
 (** We can now define antisymmetry w.r.t. an equivalence relation on the carrier. *)
 
-Class [ Equivalence A eqA ] => antisymmetric (R : relation A) := 
+Class [ Equivalence A eqA ] => Antisymmetric (R : relation A) := 
   antisymmetry : forall x y, R x y -> R y x -> eqA x y.
 
-Program Instance [ eq : Equivalence A eqA, antisymmetric eq R ] => 
-  flip_antisymmetric : antisymmetric eq (flip R).
+Program Instance [ eq : Equivalence A eqA, Antisymmetric eq R ] => 
+  flip_antiSymmetric : Antisymmetric eq (flip R).
 
-Program Instance [ eq : Equivalence A eqA, antisymmetric eq (R : relation A) ] => 
-  inverse_antisymmetric : antisymmetric eq (inverse R).
+Program Instance [ eq : Equivalence A eqA, Antisymmetric eq (R : relation A) ] => 
+  inverse_antiSymmetric : Antisymmetric eq (inverse R).
 
 (** Leibinz equality [eq] is an equivalence relation. *)
 
