theories/Classes/Functions.v
@@ -15,9 +15,8 @@
 
 (* $Id: FSetAVL_prog.v 616 2007-08-08 12:28:10Z msozeau $ *)
 
-Require Import Coq.Program.Program.
-Require Export Coq.Classes.RelationClasses.
-Require Export Coq.Classes.Morphisms.
+Require Import Coq.Classes.RelationClasses.
+Require Import Coq.Classes.Morphisms.
 
 Set Implicit Arguments.
 Unset Strict Implicit.
